cedar-lean/Cedar/SymCCOpt/Enforcer.lean
@@ -25,14 +25,14 @@ open Cedar.Data Cedar.Spec Factory
 Returns the ground acyclicity and transitivity assumptions for a single `CompiledPolicy`.
 -/
 def enforceCompiledPolicy (cp : CompiledPolicy) : Set Term :=
-  let tr := cp.footprint.elts.mapUnion (λ t => cp.footprint.elts.map (transitivity t · cp.εnv.entities))
+  let tr := cp.footprint.elts.flatMap (λ t => cp.footprint.elts.map (transitivity t · cp.εnv.entities))
   Set.make (cp.acyclicity.elts ++ tr)
 
 /--
 Returns the ground acyclicity and transitivity assumptions for a single `CompiledPolicies`.
 -/
 def enforceCompiledPolicies (cps : CompiledPolicies) : Set Term :=
-  let tr := cps.footprint.elts.mapUnion (λ t => cps.footprint.elts.map (transitivity t · cps.εnv.entities))
+  let tr := cps.footprint.elts.flatMap (λ t => cps.footprint.elts.map (transitivity t · cps.εnv.entities))
   Set.make (cps.acyclicity.elts ++ tr)
 
 /--
@@ -42,7 +42,7 @@ Caller guarantees that `cp₁` and `cp₂` were compiled for the same `εnv`.
 def enforcePairCompiledPolicy (cp₁ : CompiledPolicy) (cp₂ : CompiledPolicy) : Set Term :=
   assert! cp₁.εnv = cp₂.εnv
   let footprint := cp₁.footprint ++ cp₂.footprint
-  let tr := footprint.elts.mapUnion (λ t => footprint.elts.map (transitivity t · cp₁.εnv.entities))
+  let tr := footprint.elts.flatMap (λ t => footprint.elts.map (transitivity t · cp₁.εnv.entities))
   Set.make (cp₁.acyclicity.elts ++ cp₂.acyclicity.elts ++ tr)
 
 /--
@@ -52,7 +52,7 @@ Caller guarantees that `cps₁` and `cps₂` were compiled for the same `εnv`.
 def enforcePairCompiledPolicies (cps₁ : CompiledPolicies) (cps₂ : CompiledPolicies) : Set Term :=
   assert! cps₁.εnv = cps₂.εnv
   let footprint := cps₁.footprint ++ cps₂.footprint
-  let tr := footprint.elts.mapUnion (λ t => footprint.elts.map (transitivity t · cps₁.εnv.entities))
+  let tr := footprint.elts.flatMap (λ t => footprint.elts.map (transitivity t · cps₁.εnv.entities))
   Set.make (cps₁.acyclicity.elts ++ cps₂.acyclicity.elts ++ tr)
 
 namespace Cedar.SymCC
